Iris/Iris/Tests/WeakestPre.lean
@@ -122,15 +122,30 @@ section TestTotalTexanTriple
 
 set_option linter.unusedVariables false
 
-variable (PROP Expr Val : Type _) [BI PROP]
-variable [TotalWp PROP Expr Val Stuckness]
-variable (e : Expr) (P Q : PROP) (v : Val)
+variable (PROP Expr Val A : Type _) [BI PROP]
+variable [TotalWp PROP Expr Val A] [TotalWp PROP Expr Val Stuckness]
+variable (e : Expr) (s : A) (E : CoPset) (P Q : PROP) (v : Val)
+
+/-- info: iprop(∀ Φ, P -∗ (Q -∗ Φ v) -∗ WP e @ s ; E [{ Φ }] ) : PROP -/
+#guard_msgs in #check [[{ P }]] e @ s ; E [[{ RET v; Q }]]
+
+/-- info: iprop(∀ Φ, P -∗ (Q -∗ Φ v) -∗ WP e @ E [{ Φ }] ) : PROP -/
+#guard_msgs in #check [[{ P }]] e @ E [[{ RET v; Q }]]
+
+/-- info: iprop(∀ Φ, P -∗ (Q -∗ Φ v) -∗ WP e @ E ? [{ Φ }] ) : PROP -/
+#guard_msgs in #check [[{ P }]] e @ E ? [[{ RET v; Q }]]
 
 /-- info: iprop(∀ Φ, P -∗ (Q -∗ Φ v) -∗ WP e [{ Φ }] ) : PROP -/
 #guard_msgs in #check [[{ P }]] e [[{ RET v; Q }]]
 
+/-- info: iprop(∀ Φ, P -∗ (Q -∗ Φ v) -∗ WP e ? [{ Φ }] ) : PROP -/
+#guard_msgs in #check [[{ P }]] e ? [[{ RET v; Q }]]
+
 /-- info: iprop(∀ Φ, P -∗ (∀ x, Q -∗ Φ x) -∗ WP e [{ Φ }] ) : PROP -/
-#guard_msgs in #check [[{ P }]] e [[{ x, RET x; Q }]]
+#guard_msgs in #check [[{ P }]] e [[{ (x : Val), RET x; Q }]]
+
+/-- info: iprop(∀ Φ, P -∗ (∀ x, Q -∗ Φ v) -∗ WP e [{ Φ }] ) : PROP -/
+#guard_msgs in #check [[{ P }]] e [[{ _, RET v; Q }]]
 
 end TestTotalTexanTriple
 
